Allow adding instructions to VProg

VProg/Core.v
@@ -1202,148 +1202,6 @@ Section Call.
     Qed.
   End Ghost.
 End Call.
-Section GGet.
-  Context [A : Type] (v : Vprop.p A).
-
-  Inductive GGet_Spec (ctx : CTX.t) : i_spec_t A ctx -> Prop
-    := GGet_SpecI
-    (a : A) (csm : Sub.t ctx)
-    (ij : CTX.Inj.ieq [CTX.mka (v, a)] ctx csm):
-    GGet_Spec ctx {|
-      sf_csm  := Sub.const ctx false;
-      sf_prd  := fun _ => nil;
-      sf_spec := FP.Ret (TF.mk _ a Tuple.tt)
-    |}.
-
-  Program Definition gGet : instr A := {|
-    i_impl := CP.Oracle A;
-    i_spec := fun ctx => GGet_Spec ctx;
-  |}.
-  Next Obligation.
-    destruct SP; do 2 intro; simpl in *.
-    apply SP.COracle with (x := a).
-    Apply tt.
-    Apply. assumption.
-    unfold Sub.neg, Sub.const; rewrite Vector.map_const; cbn.
-    rewrite Sub.sub_const_true.
-    reflexivity.
-  Qed.
-End GGet.
-Section Assert.
-  Context [A : Type] (P : A -> CTX.t * Prop).
-
-  Inductive Assert_Spec (ctx : CTX.t) : i_spec_t unit ctx -> Prop
-    := Assert_SpecI
-    (p : A)
-    (img : Sub.t ctx)
-    (ij : CTX.Inj.ieq (fst (P p)) ctx img):
-    Assert_Spec ctx {|
-      sf_csm  := Sub.const ctx false;
-      sf_prd  := fun _ => nil;
-      sf_spec := FP.Bind (FP.Assert (snd (P p)))
-                         (TF.of_fun (fun _ => FP.Ret (TF.mk _ tt Tuple.tt)))
-    |}.
-  
-  Program Definition Assert : instr unit := {|
-    i_impl := SP.sl_assert (SLprop.ex A (fun p =>
-                SLprop.pure (snd (P p)) ** CTX.sl (fst (P p))))%slprop;
-    i_spec := fun ctx => Assert_Spec ctx;
-  |}.
-  Next Obligation.
-    destruct SP; do 2 intro; simpl in *.
-    case PRE as (PRE & POST).
-    eapply SP.CFrame with (fr := CTX.sl (CTX.sub ctx (Sub.neg img))).
-    - apply SP.Assert_imp with (Q := CTX.sl (fst (P p))).
-      Apply p.
-      Apply PRE.
-      reflexivity.
-    - eenough (SLprop.eq (CTX.sl ctx) _) as sl_eq.
-      split; unfold sf_post, sf_post_ctx, sf_rsel; simpl.
-      + rewrite sl_eq; reflexivity.
-      + intros []; SL.normalize.
-        Apply POST.
-        unfold Sub.neg, Sub.const; rewrite Vector.map_const; simpl.
-        rewrite Sub.sub_const_true.
-        rewrite sl_eq; reflexivity.
-      + rewrite CTX.sl_split with (s := img).
-        setoid_rewrite (CTX.Inj.ieqE ij).
-        reflexivity.
-  Qed.
-End Assert.
-Section Read.
-  Context (p : ptr).
-
-  Inductive Read_Spec (ctx : CTX.t) : i_spec_t memdata ctx -> Prop
-    := Read_SpecI
-    (d : memdata)
-    (img : Sub.t ctx)
-    (ij : CTX.Inj.ieq [CTX.mka (SLprop.cell p, d)] ctx img):
-    Read_Spec ctx {|
-      sf_csm  := Sub.const ctx false;
-      sf_prd  := fun _ => nil;
-      sf_spec := FP.Ret (TF.mk _ d Tuple.tt);
-    |}.
-
-  Program Definition Read : instr memdata := {|
-    i_impl := CP.Read p;
-    i_spec := fun ctx => Read_Spec ctx;
-  |}.
-  Next Obligation.
-    destruct SP; do 2 intro; simpl in *.
-    eapply SP.CFrame with (fr := CTX.sl (CTX.sub ctx (Sub.neg img))).
-    - eapply SP.Read with (d := d).
-    - eassert (IEq : SLprop.eq _ _). {
-        etransitivity. apply (CTX.Inj.ieqE ij).
-        simpl; SL.normalize.
-      }
-      split; simpl.
-      + rewrite CTX.sl_split with (s := img).
-        apply SLprop.star_morph_imp. 2:reflexivity.
-        rewrite IEq; reflexivity.
-      + intro. SL.normalize. Intro ->.
-        unfold sf_post; simpl; SL.normalize.
-        Apply. assumption.
-        etransitivity. apply SLprop.star_morph_imp. 2:reflexivity. 
-        eapply SLprop.imp_morph. symmetry in IEq; exact IEq. 1,2:reflexivity.
-        rewrite <- CTX.sl_split.
-        unfold Sub.neg, Sub.const; rewrite Vector.map_const; simpl.
-        rewrite Sub.sub_const_true.
-        reflexivity.
-  Qed.
-End Read.
-Section Write.
-  Context (p : ptr) (d : memdata).
-
-  Inductive Write_Spec (ctx : CTX.t) : i_spec_t unit ctx -> Prop
-    := Write_SpecI
-    (d0 : memdata)
-    (csm : Sub.t ctx)
-    (ij : CTX.Inj.ieq [CTX.mka (SLprop.cell p, d0)] ctx csm):
-    Write_Spec ctx {|
-      sf_csm  := csm;
-      sf_prd  := fun _ => [Vprop.mk (SLprop.cell p)];
-      sf_spec := FP.Ret (TF.mk (fun _ => [memdata]) tt (d, tt));
-    |}.
-
-  Program Definition Write : instr unit := {|
-    i_impl := CP.Write p d;
-    i_spec := fun ctx => Write_Spec ctx;
-  |}.
-  Next Obligation.
-    destruct SP; do 2 intro; simpl in *.
-    eapply SP.CFrame with (fr := CTX.sl (CTX.sub ctx (Sub.neg csm))).
-    - eapply SP.Write with (d0 := d0).
-    - split; unfold sf_post, sf_post_ctx, sf_rsel; simpl.
-      + rewrite CTX.sl_split with (s := csm).
-        apply SLprop.star_morph_imp. 2:reflexivity.
-        rewrite (CTX.Inj.ieqE ij); simpl; SL.normalize; reflexivity.
-      + intros []; SL.normalize.
-        Apply (d, tt).
-        Apply. assumption.
-        reflexivity.
-  Qed.
-End Write.
-
 End VProg.
 
 Global Arguments Ret [_ _] _ {pt}.
@@ -1352,10 +1210,6 @@ Global Arguments Bind [_ _ _] _ _.
 Global Arguments Call [_ _ _ _] _ _ _ [_] _.
 Global Arguments Call_f_decl [_ _ _ _] _ _.
 Global Arguments gLem [_ _ _] _ _.
-Global Arguments gGet [_ _] _.
-Global Arguments Assert [_ _].
-Global Arguments Read [_] _.
-Global Arguments Write [_] _ _.
 
 
 Module NotationsDef.
@@ -1552,6 +1406,11 @@ Module Tac.
     | (* F1   *) Tac.cbn_refl ].
 
 
+  (* Tactics to build the instruction specifications. *)
+  Global Create HintDb HasSpecDB discriminated.
+  Global Hint Constants Opaque : HasSpecDB.
+  Global Hint Variables Opaque : HasSpecDB.
+
   Ltac build_Ret :=
     simple refine (@Ret_SpecI _ _ _ _ _ _ _);
     [ Tuple.build_shape | shelve | CTX.Inj.build ].
@@ -1582,29 +1441,6 @@ Module Tac.
       CTX.Inj.build
     | shelve | (* ij_prs *) cbn; CTX.Inj.build
     | shelve | (* SF     *) cbn_refl ].
-
-  Ltac build_GGet :=
-    simple refine (GGet_SpecI _ _ _ _ _);
-    [ shelve | shelve | CTX.Inj.build ].
-
-  Ltac build_Assert :=
-    simple refine (@Assert_SpecI _ _ _ _ _ _);
-    [ shelve | shelve |
-      cbn;
-      (* [p : A] can be a tuple let-matched by [P] *)
-      repeat lazymatch goal with |- CTX.Inj.ieq (fst ?x) _ _ =>
-        build_matched_shape x; cbn
-      end;
-      (* ij *)
-      CTX.Inj.build ].
-
-  Ltac build_Read :=
-    simple refine (@Read_SpecI _ _ _ _ _);
-    [ shelve | shelve | (* ij *) CTX.Inj.build ].
-
-  Ltac build_Write :=
-    simple refine (@Write_SpecI _ _ _ _ _ _);
-    [ shelve | shelve | (* ij *) CTX.Inj.build ].
 
   (* TODO: be more careful about the dependencies on the matched term in the vprog and in the context *)
 
@@ -1675,11 +1511,8 @@ Module Tac.
         | |- Ret_Spec    _ _ _ _ => build_Ret
         | |- Bind_Spec _ _ _ _ _ => build_Bind build
         | |- Call_Spec     _ _ _ => build_Call
-        | |- GGet_Spec     _ _ _ => build_GGet
-        | |- Assert_Spec   _ _ _ => build_Assert
-        | |- Read_Spec     _ _ _ => build_Read
-        | |- Write_Spec  _ _ _ _ => build_Write
-        | |- ?g => fail "HasSpec::ct" g
+        | |- ?g => try solve [eauto 1 with HasSpecDB nocore];
+                   fail "HasSpec::ct" g
         end
     | (match ?x with _ => _ end) =>
         tryif is_single_case x
