VProg/Instructions.v
@@ -1,0 +1,95 @@
+From SLFun Require Import Util Values SL VProg.Vprop VProg.Core.
+From Coq   Require Import Lists.List.
+
+Import ListNotations SLNotations VProg.Core.Abbrev.
+Import SL.Tactics.
+
+
+Section Read.
+  Context [CT : CP.context] (p : ptr).
+
+  Inductive Read_Spec (ctx : CTX.t) : i_spec_t memdata ctx -> Prop
+    := Read_SpecI
+    (d : memdata)
+    (img : Sub.t ctx)
+    (ij : CTX.Inj.ieq [CTX.mka (SLprop.cell p, d)] ctx img):
+    Read_Spec ctx {|
+      sf_csm  := Sub.const ctx false;
+      sf_prd  := fun _ => nil;
+      sf_spec := FP.Ret (TF.mk _ d Tuple.tt);
+    |}.
+
+  Program Definition Read : instr CT memdata := {|
+    i_impl := CP.Read p;
+    i_spec := fun ctx => Read_Spec ctx;
+  |}.
+  Next Obligation.
+    destruct SP; do 2 intro; simpl in *.
+    eapply SP.CFrame with (fr := CTX.sl (CTX.sub ctx (Sub.neg img))).
+    - eapply SP.Read with (d := d).
+    - eassert (IEq : SLprop.eq _ _). {
+        etransitivity. apply (CTX.Inj.ieqE ij).
+        simpl; SL.normalize.
+      }
+      split; simpl.
+      + rewrite CTX.sl_split with (s := img).
+        apply SLprop.star_morph_imp. 2:reflexivity.
+        rewrite IEq; reflexivity.
+      + intro. SL.normalize. Intro ->.
+        unfold sf_post; simpl; SL.normalize.
+        Apply. assumption.
+        etransitivity. apply SLprop.star_morph_imp. 2:reflexivity. 
+        eapply SLprop.imp_morph. symmetry in IEq; exact IEq. 1,2:reflexivity.
+        rewrite <- CTX.sl_split.
+        unfold Sub.neg, Sub.const; rewrite Vector.map_const; simpl.
+        rewrite Sub.sub_const_true.
+        reflexivity.
+  Qed.
+End Read.
+
+Local Ltac build_Read :=
+  simple refine (@Read_SpecI _ _ _ _ _);
+  [ shelve | shelve | (* ij *) CTX.Inj.build ].
+
+Section Write.
+  Context [CT : CP.context] (p : ptr) (d : memdata).
+
+  Inductive Write_Spec (ctx : CTX.t) : i_spec_t unit ctx -> Prop
+    := Write_SpecI
+    (d0 : memdata)
+    (csm : Sub.t ctx)
+    (ij : CTX.Inj.ieq [CTX.mka (SLprop.cell p, d0)] ctx csm):
+    Write_Spec ctx {|
+      sf_csm  := csm;
+      sf_prd  := fun _ => [Vprop.mk (SLprop.cell p)];
+      sf_spec := FP.Ret (TF.mk (fun _ => [memdata]) tt (d, tt));
+    |}.
+
+  Program Definition Write : instr CT unit := {|
+    i_impl := CP.Write p d;
+    i_spec := fun ctx => Write_Spec ctx;
+  |}.
+  Next Obligation.
+    destruct SP; do 2 intro; simpl in *.
+    eapply SP.CFrame with (fr := CTX.sl (CTX.sub ctx (Sub.neg csm))).
+    - eapply SP.Write with (d0 := d0).
+    - split; unfold sf_post, sf_post_ctx, sf_rsel; simpl.
+      + rewrite CTX.sl_split with (s := csm).
+        apply SLprop.star_morph_imp. 2:reflexivity.
+        rewrite (CTX.Inj.ieqE ij); simpl; SL.normalize; reflexivity.
+      + intros []; SL.normalize.
+        Apply (d, tt).
+        Apply. assumption.
+        reflexivity.
+  Qed.
+End Write.
+
+Local Ltac build_Write :=
+  simple refine (@Write_SpecI _ _ _ _ _ _);
+  [ shelve | shelve | (* ij *) CTX.Inj.build ].
+
+Module Tactics.
+  #[export] Hint Extern 1 (Read_Spec    _ _ _) => build_Read   : HasSpecDB.
+  #[export] Hint Extern 1 (Write_Spec _ _ _ _) => build_Write  : HasSpecDB.
+End Tactics.
+Export Tactics.
