VProg/Main.v
@@ -1,8 +1,8 @@
-From SLFun.VProg Require Export Vprop Core Ghost.
+From SLFun.VProg Require Export Vprop Core Ghost Instructions.
 
 Module Tactics.
   Export ConcreteProg.Tactics.
-  Export VProg.Core.Tactics.
+  Export VProg.Core.Tactics VProg.Ghost.Tactics VProg.Instructions.Tactics.
 End Tactics.
 
 Module Notations.
